Work on making arrows only need a single index

src/Solver.v
@@ -15,6 +15,23 @@ Require Import Coq.PArith.PArith.
 
 Generalizable All Variables.
 
+Open Scope lazy_bool_scope.
+
+Definition rev_list_rect (A : Type) (P : list A → Type) (H : P [])
+           (H0 : ∀ (a : A) (l : list A), P (rev l) → P (rev (a :: l)))
+           (l : list A) : P (rev l) :=
+  list_rect (λ l0 : list A, P (rev l0)) H
+            (λ (a : A) (l0 : list A) (IHl : P (rev l0)), H0 a l0 IHl) l.
+
+Definition rev_rect (A : Type) (P : list A → Type)
+           (H : P []) (H0 : ∀ (x : A) (l : list A), P l → P (l ++ [x]))
+           (l : list A) : P l :=
+  (λ E : rev (rev l) = l,
+     eq_rect (rev (rev l)) (λ l0 : list A, P l0)
+        (rev_list_rect A P H
+        (λ (a : A) (l0 : list A) (H1 : P (rev l0)), H0 a (rev l0) H1)
+        (rev l)) l E) (rev_involutive l).
+
 Lemma last_rcons A (x y : A) l :
   last (l ++ [x]) y = x.
 Proof.
@@ -48,6 +65,16 @@ Proof.
   destruct ys; auto.
 Qed.
 
+Lemma match_last {A} {a : A} {xs x} :
+  match xs with
+  | [] => a
+  | _ :: _ => last xs x
+  end = last xs a.
+Proof.
+  induction xs; auto.
+  rewrite !last_cons; reflexivity.
+Qed.
+
 Lemma Forall_app {A} p (l1 l2: list A) :
   Forall p (l1 ++ l2) <-> (Forall p l1 /\ Forall p l2).
 Proof.
@@ -73,114 +100,6 @@ Proof.
   destruct H0.
   now inversion H0.
 Qed.
-
-Definition cat_idx := positive.
-Definition obj_idx := positive.
-Definition arr_idx := positive.
-
-Set Universe Polymorphism.
-
-Program Instance option_setoid `{Setoid A} : Setoid (option A) := {
-  equiv := fun x y => match x, y with
-    | Some x, Some y => x ≈ y
-    | None, None => True
-    | _, _ => False
-    end
-}.
-Next Obligation. intuition; discriminate. Qed.
-Next Obligation. intuition; discriminate. Qed.
-Next Obligation.
-  equivalence.
-  - destruct x; reflexivity.
-  - destruct x, y; auto.
-    symmetry; auto.
-  - destruct x, y, z; auto.
-      transitivity a0; auto.
-    contradiction.
-Qed.
-
-Unset Universe Polymorphism.
-
-Open Scope positive_scope.
-
-(* This describes the morphisms of a magmoid, which forms a quotient category
-   under denotation. *)
-Inductive Term : Set :=
-  | Identity : cat_idx -> obj_idx -> Term
-  | Morph    : cat_idx -> obj_idx -> obj_idx -> arr_idx -> Term
-  | Compose  : Term -> Term -> Term.
-
-Fixpoint TermCat (e : Term) : cat_idx :=
-  match e with
-  | Identity x _  => x
-  | Morph x _ _ _ => x
-  | Compose f _ => TermCat f
-  end.
-
-Fixpoint TermDom (e : Term) : obj_idx :=
-  match e with
-  | Identity _ x  => x
-  | Morph _ x _ _ => x
-  | Compose _ g => TermDom g
-  end.
-
-Fixpoint TermCod (e : Term) : obj_idx :=
-  match e with
-  | Identity _ x  => x
-  | Morph _ _ x _ => x
-  | Compose f _ => TermCod f
-  end.
-
-Section Denotation.
-
-Inductive Arrow : Set :=
-  | Arr : cat_idx -> obj_idx -> obj_idx -> arr_idx -> Arrow.
-
-Open Scope lazy_bool_scope.
-
-Fixpoint Arrow_beq (x y : Arrow) {struct x} : bool :=
-  match x with
-  | Arr cat dom cod arr =>
-      match y with
-      | Arr cat' dom' cod' arr' =>
-        (cat =? cat') &&& (dom =? dom') &&& (cod =? cod') &&& (arr =? arr')
-      end
-  end.
-
-Lemma Arrow_beq_eq x y :
-  Arrow_beq x y = true -> x = y.
-Proof.
-  destruct x, y; simpl.
-  intros.
-  destruct (c  =? c0) eqn:?; [|discriminate].
-  destruct (o  =? o1) eqn:?; [|discriminate].
-  destruct (o0 =? o2) eqn:?; [|discriminate].
-  destruct (a  =? a0) eqn:?; [|discriminate].
-  apply Peqb_true_eq in Heqb.
-  apply Peqb_true_eq in Heqb0.
-  apply Peqb_true_eq in Heqb1.
-  apply Peqb_true_eq in Heqb2.
-  subst; reflexivity.
-Qed.
-
-Definition Arrow_cat (f : Arrow) : cat_idx :=
-  match f with Arr x _ _ _ => x end.
-
-Definition Arrow_dom (f : Arrow) : obj_idx :=
-  match f with Arr _ x _ _ => x end.
-
-Definition Arrow_cod (f : Arrow) : obj_idx :=
-  match f with Arr _ _ y _ => y end.
-
-(* This describes the morphisms of a path, or free, category over a quiver of
-   Arrows, while our environment describes a quiver (where vertices are all
-   object indices, and edges are all arrow indices associated pairs of object
-   indices). The denotation of an ArrowList to some category C is a forgetful
-   functor from the path category over this quiver to C. Note that this
-   functor is only total if the denotation of the quiver itself is total. *)
-Inductive ArrowList : Set :=
-  | IdentityOnly : cat_idx -> obj_idx -> ArrowList
-  | ArrowChain   : Arrow -> list Arrow -> ArrowList.
 
 Fixpoint list_beq {A : Type} (eq_A : A → A → bool) (X Y : list A)
          {struct X} : bool :=
@@ -211,106 +130,13 @@ Proof.
   discriminate.
 Qed.
 
-Fixpoint ArrowList_beq  (x y : ArrowList) {struct x} : bool :=
-  match x with
-  | IdentityOnly cat cod =>
-      match y with
-      | IdentityOnly cat' cod' => (cat =? cat') &&& (cod =? cod')
-      | ArrowChain _ _ => false
-      end
-  | ArrowChain x x0 =>
-      match y with
-      | IdentityOnly _ _ => false
-      | ArrowChain x1 x2 => Arrow_beq x x1 &&& list_beq Arrow_beq x0 x2
-      end
-  end.
-
-Definition ArrowList_cat (xs : ArrowList) : cat_idx :=
-  match xs with
-  | IdentityOnly x _ => x
-  | ArrowChain (Arr x _ _ _) _ => x
-  end.
-
-Definition ArrowList_cod (xs : ArrowList) : obj_idx :=
-  match xs with
-  | IdentityOnly _ x => x
-  | ArrowChain (Arr _ x y f) _ => y
-  end.
-
-Definition ArrowList_dom (xs : ArrowList) : obj_idx :=
-  match xs with
-  | IdentityOnly _ x => x
-  | ArrowChain f xs =>
-    match last xs f with
-    | Arr _ x y m => x
-    end
-  end.
-
-Inductive ForallAligned : list Arrow → Prop :=
-    Align_nil : ForallAligned []
-  | Align_singleton : ∀ (a : Arrow), ForallAligned [a]
-  | Align_cons2 : ∀ (a b : Arrow) (l : list Arrow),
-      Arrow_dom a = Arrow_cod b ->
-      ForallAligned (b :: l) → ForallAligned (a :: b :: l).
-
-Lemma ForallAligned_inv {x xs y} :
-  ForallAligned (x :: y :: xs)
-    -> Arrow_dom x = Arrow_cod y /\ ForallAligned (y :: xs).
+Lemma list_beq_refl {A} (R : A -> A -> bool) xs :
+  (∀ x, R x x = true) -> list_beq R xs xs = true.
 Proof.
-  generalize dependent x.
-  generalize dependent y.
-  induction xs; intros;
-  inversion H; subst; intuition.
+  intros.
+  induction xs; auto; simpl.
+  now rewrite H.
 Qed.
-
-Lemma match_last {A} {a : A} {xs x} :
-  match xs with
-  | [] => a
-  | _ :: _ => last xs x
-  end = last xs a.
-Proof.
-  induction xs; auto.
-  rewrite !last_cons; reflexivity.
-Qed.
-
-Lemma ForallAligned_app {x xs y ys} :
-  ForallAligned (x :: xs ++ y :: ys)
-    <-> ForallAligned (x :: xs) /\ ForallAligned (y :: ys) /\
-        Arrow_cod y = Arrow_dom (last xs x).
-Proof.
-  generalize dependent x.
-  generalize dependent y.
-  generalize dependent ys.
-  induction xs; simpl; intros.
-    split; intros.
-      inversion H.
-      split; constructor; auto.
-    constructor; auto; intuition.
-  specialize (IHxs ys y a).
-  intuition;
-  try (apply ForallAligned_inv in H0;
-       destruct H0;
-       specialize (H H2)).
-  - constructor; intuition.
-  - intuition.
-  - rewrite match_last; intuition.
-  - inversion H2.
-    rewrite match_last in H4.
-    constructor; intuition.
-Qed.
-
-Definition ArrowList_well_typed cat dom cod (xs : ArrowList) : Prop :=
-  match xs with
-  | IdentityOnly c x => c = cat /\ x = dom /\ x = cod
-  | ArrowChain (Arr c x y f) xs =>
-    y = cod /\
-    match last xs (Arr c x y f) with
-      Arr c' a b g => c = c' /\ a = dom
-    end /\
-    (* Ensure that it is a correctly type-aligned list *)
-    Forall (fun '(Arr c x y f) => c = cat) (Arr c x y f :: xs) /\
-    ForallAligned (Arr c x y f :: xs)
-  end.
 
 Lemma K_dec_on_type A (x : A) (eq_dec : ∀ y : A, x = y \/ x ≠ y)
       (P : x = x -> Type) :
@@ -337,9 +163,244 @@ Proof.
   contradiction.
 Qed.
 
+Lemma Fin_eq_dec' : ∀ n (x y : Fin.t n), x = y \/ x ≠ y.
+Proof.
+  intros.
+  destruct (Fin.eq_dec x y); auto.
+Qed.
+
+Lemma Fin_eq_dec_refl n (x : Fin.t n) :
+  Fin.eq_dec x x = left (@eq_refl (Fin.t n) x).
+Proof.
+  destruct (Fin.eq_dec x x).
+    refine (K_dec_on_type (Fin.t n) x (Fin_eq_dec' n x)
+              (fun H => @left _ _ H = @left _ _ (@eq_refl (Fin.t n) x)) _ _).
+    reflexivity.
+  contradiction.
+Qed.
+
+Lemma Fin_eqb_refl n (x : Fin.t n) : Fin.eqb x x = true.
+Proof.
+  now apply Fin.eqb_eq.
+Qed.
+
+Set Universe Polymorphism.
+
+Program Instance option_setoid `{Setoid A} : Setoid (option A) := {
+  equiv := fun x y => match x, y with
+    | Some x, Some y => x ≈ y
+    | None, None => True
+    | _, _ => False
+    end
+}.
+Next Obligation. intuition; discriminate. Qed.
+Next Obligation. intuition; discriminate. Qed.
+Next Obligation.
+  equivalence.
+  - destruct x; reflexivity.
+  - destruct x, y; auto.
+    symmetry; auto.
+  - destruct x, y, z; auto.
+      transitivity a0; auto.
+    contradiction.
+Qed.
+
+Unset Universe Polymorphism.
+
+Open Scope positive_scope.
+
+Section Denotation.
+
+Import EqNotations.
+
+Record Vars := {
+  vars_cat : Category;
+
+  vars_num_objs : nat;
+  vars_num_arrs : nat;
+
+  vars_objs : Vector.t vars_cat vars_num_objs;
+
+  vars_arrs :
+    Vector.t (∃ (dom cod : Fin.t vars_num_objs),
+                 Vector.nth vars_objs dom ~{vars_cat}~>
+                 Vector.nth vars_objs cod)
+             vars_num_arrs
+}.
+
+Record Environment := {
+  num_cats : nat;
+  _cat_idx := Fin.t num_cats;
+
+  cats : Vector.t Vars num_cats;
+
+  get_cat (c : _cat_idx) := Vector.nth cats c;
+
+  _obj_idx (c : _cat_idx) := Fin.t (vars_num_objs (get_cat c));
+  _arr_idx (c : _cat_idx) := Fin.t (vars_num_arrs (get_cat c));
+
+  get_obj_cat c (o : _obj_idx c) := c;
+  get_obj     c (o : _obj_idx c) := Vector.nth (vars_objs (get_cat c)) o;
+
+  get_arr_cat c (a : _arr_idx c) := c;
+  get_arr_dom c (a : _arr_idx c) := `1 (Vector.nth (vars_arrs (get_cat c)) a);
+  get_arr_cod c (a : _arr_idx c) := `1 `2 (Vector.nth (vars_arrs (get_cat c)) a);
+  get_arr     c (a : _arr_idx c) := `2 `2 (Vector.nth (vars_arrs (get_cat c)) a)
+}.
+
+Variable env : Environment.
+Variable c : _cat_idx env.
+
+Arguments num_cats {_}.
+Notation cat_idx := (_cat_idx env).
+Arguments cats {_}.
+Arguments get_cat {_} _.
+Notation obj_idx := (_obj_idx env c).
+Notation arr_idx := (_arr_idx env c).
+Arguments get_obj_cat {_ _} _.
+Arguments get_obj {_ _} _.
+Arguments get_arr_cat {_ _} _.
+Arguments get_arr_dom {_ _} _.
+Arguments get_arr_cod {_ _} _.
+Arguments get_arr {_ _} _.
+
+(* This describes the morphisms of a magmoid, which forms a quotient category
+   under denotation. *)
+Inductive Term : Set :=
+  | Identity (o : obj_idx)
+  | Morph    (a : arr_idx)
+  | Compose  (f g : Term).
+
+Fixpoint TermCat (e : Term) : cat_idx :=
+  match e with
+  | Identity  _ => c
+  | Morph _     => c
+  | Compose f _ => TermCat f
+  end.
+
+Fixpoint TermDom (e : Term) : obj_idx :=
+  match e with
+  | Identity x  => x
+  | Morph x     => get_arr_dom x
+  | Compose _ g => TermDom g
+  end.
+
+Fixpoint TermCod (e : Term) : obj_idx :=
+  match e with
+  | Identity x  => x
+  | Morph x     => get_arr_cod x
+  | Compose f _ => TermCod f
+  end.
+
+Definition Arrow := arr_idx.
+
+Definition Arrow_beq (x y : Arrow) : bool := Fin.eqb x y.
+
+Lemma Arrow_beq_eq (x y : Arrow) : Arrow_beq x y = true -> x = y.
+Proof. intros; now apply Fin.eqb_eq. Qed.
+
+Lemma Arrow_beq_refl (x : Arrow) : Arrow_beq x x = true.
+Proof. intros; now apply Fin.eqb_eq. Qed.
+
+(* This describes the morphisms of a path, or free, category over a quiver of
+   Arrows, while our environment describes a quiver (where vertices are all
+   object indices, and edges are all arrow indices associated pairs of object
+   indices). The denotation of an ArrowList to some category C is a forgetful
+   functor from the path category over this quiver to C. Note that this
+   functor is only total if the denotation of the quiver itself is total. *)
+Inductive ArrowList : Set :=
+  | IdentityOnly : obj_idx -> ArrowList
+  | ArrowChain   : Arrow -> list Arrow -> ArrowList.
+
+Fixpoint ArrowList_beq (x y : ArrowList) {struct x} : bool :=
+  match x with
+  | IdentityOnly cod =>
+      match y with
+      | IdentityOnly cod' => Fin.eqb cod cod'
+      | ArrowChain _ _ => false
+      end
+  | ArrowChain x x0 =>
+      match y with
+      | IdentityOnly _ => false
+      | ArrowChain x1 x2 => Arrow_beq x x1 &&& list_beq Arrow_beq x0 x2
+      end
+  end.
+
+Definition ArrowList_cat (xs : ArrowList) : cat_idx :=
+  match xs with
+  | IdentityOnly x => c
+  | ArrowChain f _ => c
+  end.
+
+Definition ArrowList_cod (xs : ArrowList) : obj_idx :=
+  match xs with
+  | IdentityOnly x => x
+  | ArrowChain f _ => get_arr_cod f
+  end.
+
+Definition ArrowList_dom (xs : ArrowList) : obj_idx :=
+  match xs with
+  | IdentityOnly x => x
+  | ArrowChain f xs => get_arr_dom (last xs f)
+  end.
+
+Inductive ForallAligned : list Arrow → Prop :=
+    Align_nil : ForallAligned []
+  | Align_singleton : ∀ (a : Arrow), ForallAligned [a]
+  | Align_cons2 : ∀ (a b : Arrow) (l : list Arrow),
+      get_arr_dom a = get_arr_cod b ->
+      ForallAligned (b :: l) → ForallAligned (a :: b :: l).
+
+Lemma ForallAligned_inv {x xs y} :
+  ForallAligned (x :: y :: xs)
+    -> get_arr_dom x = get_arr_cod y /\
+       ForallAligned (y :: xs).
+Proof.
+  generalize dependent x.
+  generalize dependent y.
+  induction xs; intros;
+  inversion H; subst; intuition.
+Qed.
+
+Lemma ForallAligned_app {x xs y ys} :
+  ForallAligned (x :: xs ++ y :: ys)
+    <-> ForallAligned (x :: xs) /\ ForallAligned (y :: ys) /\
+        get_arr_cod y = get_arr_dom (last xs x).
+Proof.
+  generalize dependent x.
+  generalize dependent y.
+  generalize dependent ys.
+  induction xs; simpl; intros.
+    split; intros.
+      inversion H.
+      split; constructor; auto.
+    constructor; auto; intuition.
+  specialize (IHxs ys y a).
+  intuition;
+  try (apply ForallAligned_inv in H0;
+       destruct H0;
+       specialize (H H2)).
+  - constructor; intuition.
+  - intuition.
+  - rewrite match_last; intuition.
+  - inversion H2.
+    rewrite match_last in H4.
+    constructor; intuition.
+Qed.
+
+Definition ArrowList_well_typed dom cod (xs : ArrowList) : Prop :=
+  match xs with
+  | IdentityOnly x => x = dom /\ x = cod
+  | ArrowChain f xs =>
+    get_arr_cod f = cod /\
+    get_arr_dom (last xs f) = dom /\
+    (* Ensure that it is a correctly type-aligned list *)
+    ForallAligned (f :: xs)
+  end.
+
 Ltac equalities :=
   repeat (
-    lazymatch goal with
+    match goal with
     | [ H : context[match Pos.eq_dec ?N ?N with _ => _ end] |- _ ] =>
       rewrite Neq_dec_refl in H
     | [ |- context[match Pos.eq_dec ?N ?N with _ => _ end] ] =>
@@ -353,59 +414,48 @@ Ltac equalities :=
     | [ |- context[if ?N =? ?M then _ else _] ] =>
       let Heqe := fresh "Heqe" in
       destruct (N =? M) eqn:Heqe
-    | [ H : (_ &&& _) = true |- _ ] =>
-      rewrite <- andb_lazy_alt in H
-    | [ H : (_ && _) = true |- _ ] =>
-      apply andb_true_iff in H;
-      destruct H
-    | [ H : _ /\ _ |- _ ] =>
-      destruct H
-    | [ H : _ ∧ _ |- _ ] =>
-      destruct H
-    | [ H : (_ =? _) = true |- _ ] =>
-      apply Pos.eqb_eq in H; subst
-    | [ H : (_ =? _) = false |- _ ] =>
-      apply Pos.eqb_neq in H
+    | [ H : context[match @Fin.eq_dec ?N ?X ?X with _ => _ end] |- _ ] =>
+      rewrite (@Fin_eq_dec_refl N X) in H
+    | [ |- context[match @Fin.eq_dec ?N ?X ?X with _ => _ end] ] =>
+      rewrite (@Fin_eq_dec_refl N X)
+    | [ H : context[match @Fin.eq_dec ?N ?X ?Y with _ => _ end] |- _ ] =>
+      destruct (@Fin.eq_dec N X Y); subst
+    | [ |- context[match Fin.eq_dec ?N ?X ?Y with _ => _ end] ] =>
+      destruct (@Fin.eq_dec N X Y); subst
+    | [ |- context[Arrow_beq ?N ?N = true] ] => rewrite Arrow_beq_refl
+    | [ H : (_ &&& _) = true |- _ ]          => rewrite <- andb_lazy_alt in H
+    | [ H : (_ && _) = true |- _ ]           => apply andb_true_iff in H; destruct H
+    | [ H : _ /\ _ |- _ ]                    => destruct H
+    | [ H : _ ∧ _ |- _ ]                     => destruct H
+    | [ H : Arrow_beq _ _   = true |- _ ]    => apply Arrow_beq_eq in H
+    | [ |- Arrow_beq _ _    = true ]         => apply Arrow_beq_eq
+    | [ H : list_beq _ _ _   = true |- _ ]   => apply list_beq_eq in H
+    | [ |- list_beq _ _ _    = true ]        => apply list_beq_eq
+    | [ H : Fin.eqb _ _   = true |- _ ]      => apply Fin.eqb_eq in H
+    | [ |- Fin.eqb _ _    = true ]           => apply Fin.eqb_eq
+    | [ H : (_ =? _) = true |- _ ]           => apply Pos.eqb_eq in H
+    | [ |- (_ =? _) = true ]                 => apply Pos.eqb_eq
+    | [ H : (_ =? _) = false |- _ ]          => apply Pos.eqb_neq in H
+    | [ |- (_ =? _) = false ]                => apply Pos.eqb_neq
     end;
     subst; simpl; auto;
+    simpl TermCat in *;
     simpl TermDom in *;
     simpl TermCod in *;
     try discriminate;
     try tauto;
     try intuition idtac).
 
-Corollary ArrowList_well_typed_cat {f cat dom cod } :
-  ArrowList_well_typed cat dom cod f ->
-    match f with
-    | IdentityOnly c _ => c = cat
-    | ArrowChain (Arr c _ _ _) xs =>
-      c = cat /\ Forall (fun '(Arr c x y f) => c = cat) xs
-    end.
-Proof.
-  induction f; simpl; intros; intuition.
-  destruct a; equalities.
-    destruct (last l (Arr c o cod a)); auto.
-    now inversion H0.
-  now inversion H0.
-Qed.
+Corollary ArrowList_well_typed_dom {f dom cod } :
+  ArrowList_well_typed dom cod f -> ArrowList_dom f = dom.
+Proof. induction f; simpl; intuition. Qed.
 
-Corollary ArrowList_well_typed_dom {f cat dom cod } :
-  ArrowList_well_typed cat dom cod f -> ArrowList_dom f = dom.
-Proof.
-  induction f; simpl; intros; intuition.
-  destruct a; equalities.
-  destruct (last l (Arr c o cod a)); intuition.
-Qed.
-
-Corollary ArrowList_well_typed_cod {f cat dom cod} :
-  ArrowList_well_typed cat dom cod f -> ArrowList_cod f = cod.
-Proof.
-  induction f; simpl; intros; intuition.
-  destruct a; equalities.
-Qed.
+Corollary ArrowList_well_typed_cod {f dom cod} :
+  ArrowList_well_typed dom cod f -> ArrowList_cod f = cod.
+Proof. induction f; simpl; intuition. Qed.
 
 Definition ArrowList_list_rect : ∀ (P : ArrowList → Type),
-  (∀ (c : cat_idx) (x : obj_idx), P (IdentityOnly c x)) →
+  (∀ (x : obj_idx), P (IdentityOnly x)) →
   (∀ (a : Arrow), P (ArrowChain a [])) →
   (∀ (a1 a2 : Arrow) (l : list Arrow),
       P (ArrowChain a2 l) → P (ArrowChain a1 (a2 :: l))) →
@@ -426,30 +476,15 @@ Proof.
   - equalities.
   - inversion_clear H.
     equalities.
-    now apply Pos.eqb_eq.
-  - destruct (Arrow_beq a a0) eqn:?; [|discriminate].
-    apply Arrow_beq_eq in Heqb; subst.
-    destruct l; now auto.
+  - equalities.
+    destruct l; congruence.
   - inversion_clear H.
-    assert (∀ x, Arrow_beq x x = true).
-      destruct x; simpl.
-      now rewrite !Pos.eqb_refl.
-    now rewrite H.
-  - destruct (Arrow_beq a1 a) eqn:?; [|discriminate].
-    apply Arrow_beq_eq in Heqb; subst.
-    destruct l0; [discriminate|].
-    destruct (Arrow_beq a2 a0) eqn:?; [|discriminate].
-    apply Arrow_beq_eq in Heqb; subst.
-    apply list_beq_eq in H; subst; auto.
-    apply Arrow_beq_eq.
+    now rewrite Arrow_beq_refl.
+  - equalities.
+    destruct l0; equalities; intuition.
   - inversion_clear H.
-    assert (∀ x, Arrow_beq x x = true).
-      destruct x; simpl.
-      now rewrite !Pos.eqb_refl.
-    rewrite !H.
-    clear -H.
-    induction l; simpl; auto.
-    now rewrite H.
+    rewrite !Arrow_beq_refl, list_beq_refl; auto; intros.
+    apply Arrow_beq_refl.
 Qed.
 
 Definition ListOfArrows_rect : ∀ (P : Arrow -> list Arrow → Type),
@@ -464,14 +499,10 @@ Defined.
 
 Definition ArrowList_append (xs ys : ArrowList) : ArrowList :=
   match xs, ys with
-  | IdentityOnly _ f, IdentityOnly c r =>
-    IdentityOnly c r
-  | IdentityOnly _ f, ArrowChain (Arr c x y g) xs =>
-    ArrowChain (Arr c x y g) xs
-  | ArrowChain f xs, IdentityOnly _ g =>
-    ArrowChain f xs
-  | ArrowChain f xs, ArrowChain (Arr c z w g) ys =>
-    ArrowChain f (xs ++ Arr c z w g :: ys)
+  | IdentityOnly f,  IdentityOnly g  => IdentityOnly g
+  | IdentityOnly f,  ArrowChain g xs => ArrowChain g xs
+  | ArrowChain f xs, IdentityOnly g  => ArrowChain f xs
+  | ArrowChain f xs, ArrowChain g ys => ArrowChain f (xs ++ g :: ys)
   end.
 
 Lemma ArrowList_append_chains a a0 l l0 :
@@ -482,20 +513,15 @@ Proof.
   generalize dependent a0.
   generalize dependent l0.
   simpl.
-  induction l using rev_ind; simpl; intros.
-    destruct a0, a; subst.
-    reflexivity.
-  rewrite last_app_cons in H; simpl in H.
-  destruct x, a0, a.
-  reflexivity.
+  induction l using rev_ind; simpl; intros; auto.
 Qed.
 
-Lemma ArrowList_append_well_typed {cat dom mid cod f1 f2} :
+Lemma ArrowList_append_well_typed {dom mid cod f1 f2} :
   ArrowList_dom f1 = mid ->
   ArrowList_cod f2 = mid ->
-  ArrowList_well_typed cat mid cod f1 ->
-  ArrowList_well_typed cat dom mid f2 ->
-    ArrowList_well_typed cat dom cod (ArrowList_append f1 f2).
+  ArrowList_well_typed mid cod f1 ->
+  ArrowList_well_typed dom mid f2 ->
+    ArrowList_well_typed dom cod (ArrowList_append f1 f2).
 Proof.
   generalize dependent mid.
   generalize dependent f2.
@@ -503,143 +529,89 @@ Proof.
   - simpl in *.
     equalities; subst.
     destruct f2 using ArrowList_list_rect; simpl in *; auto.
-      destruct a; auto.
-    destruct a1, a2; auto.
-  - destruct a.
-    simpl in *; equalities; subst.
+  - simpl in *; equalities; subst.
     destruct f2.
       simpl in *; subst; intuition.
-    destruct a0.
     simpl in *; equalities.
     + induction l using rev_ind.
         simpl in *; equalities.
         inversion H2; subst.
         now inversion H.
-      destruct x.
       rewrite !last_app_cons in *; simpl in *.
-      intuition.
-        replace (match l ++ [Arr c1 o1 o2 a1] with
-                 | [] => Arr c0 o o0 a0
-                 | _ :: _ => Arr c1 o1 o2 a1
-                 end) with (Arr c1 o1 o2 a1) by (destruct l; auto).
-      constructor; auto.
-      inversion H2; subst.
-      now inversion H.
-    + constructor; auto.
-      now inversion H.
+      replace (match l ++ [x] with
+               | [] => a0
+               | _ :: _ => x
+               end) with x by (destruct l; auto); auto.
     + constructor; auto.
   - clear IHf1.
-    destruct a1, a2.
     equalities; subst.
     destruct f2.
       constructor; simpl in H1; intuition.
-      simpl in *; subst.
-      intuition.
-      rewrite <- H2.
-      destruct l; auto.
+      simpl in *; subst; intuition.
     rewrite ArrowList_append_chains by congruence.
     simpl; constructor.
       simpl in H1; intuition.
     rewrite last_app_cons, last_cons.
-    pose proof (ArrowList_well_typed_cat H1) as H3.
-    pose proof (ArrowList_well_typed_cat H2) as H4.
     pose proof (ArrowList_well_typed_dom H2) as H5.
-    simpl in H3, H4, H5.
-    replace (match l ++ a1 :: l0 with
-             | [] => Arr c0 o1 o2 a0
-             | _ :: _ => last l0 a1
-             end) with (last l0 a1) by (destruct l; auto).
-    split.
-      destruct (last l0 a1) eqn:?c, a1; intuition; subst.
-      symmetry.
-      now sapply (last_Forall _ _ _ _ _ c1 H7).
-    split.
-      clear -H3 H4.
-      destruct a1; intuition; subst.
-      inversion H0; subst.
-      do 2 constructor; auto.
-      apply Forall_app.
-      split; auto.
-    clear -H1 H2.
-    inversion H1.
-    simpl in H2.
-    rewrite 2!app_comm_cons.
+    simpl in H5.
+    replace (match l ++ a :: l0 with
+             | [] => a2
+             | _ :: _ => last l0 a
+             end) with (last l0 a) by (destruct l; auto);
+    intuition; rewrite !app_comm_cons.
     apply ForallAligned_app.
-    destruct a1; intuition; subst.
+    inversion H1.
+    inversion H2.
+    intuition.
 Qed.
 
-Definition rev_list_rect (A : Type) (P : list A → Type) (H : P [])
-           (H0 : ∀ (a : A) (l : list A), P (rev l) → P (rev (a :: l)))
-           (l : list A) : P (rev l) :=
-  list_rect (λ l0 : list A, P (rev l0)) H
-            (λ (a : A) (l0 : list A) (IHl : P (rev l0)), H0 a l0 IHl) l.
-
-Definition rev_rect (A : Type) (P : list A → Type)
-           (H : P []) (H0 : ∀ (x : A) (l : list A), P l → P (l ++ [x]))
-           (l : list A) : P l :=
-  (λ E : rev (rev l) = l,
-     eq_rect (rev (rev l)) (λ l0 : list A, P l0)
-        (rev_list_rect A P H
-        (λ (a : A) (l0 : list A) (H1 : P (rev l0)), H0 a (rev l0) H1)
-        (rev l)) l E) (rev_involutive l).
-
 (* A term is valid constructed if composition composes compatible types. *)
-Fixpoint Term_well_typed cat dom cod (e : Term) : Prop :=
+Fixpoint Term_well_typed dom cod (e : Term) : Prop :=
   match e with
-  | Identity c x  => c = cat /\ x = dom /\ x = cod
-  | Morph c x y f => c = cat /\ x = dom /\ y = cod
+  | Identity x => x = dom /\ x = cod
+  | Morph f => get_arr_dom f = dom /\ get_arr_cod f = cod
   | Compose f g =>
-    (* TermDom g = dom /\ *)
-    (* TermCod f = cod /\ *)
     TermCod g = TermDom f /\
-    Term_well_typed cat (TermCod g) cod f /\
-    Term_well_typed cat dom (TermCod g) g
+    Term_well_typed (TermCod g) cod f /\
+    Term_well_typed dom (TermCod g) g
   end.
 
-Fixpoint Term_well_typed_bool cat dom cod (e : Term) : bool :=
+Fixpoint Term_well_typed_bool dom cod (e : Term) : bool :=
   match e with
-  | Identity c x  => (c =? cat) &&& (x =? dom) &&& (x =? cod)
-  | Morph c x y f => (c =? cat) &&& (x =? dom) &&& (y =? cod)
+  | Identity x => (Fin.eqb x dom) &&& (Fin.eqb x cod)
+  | Morph f => (Fin.eqb (get_arr_dom f) dom) &&& (Fin.eqb (get_arr_cod f) cod)
   | Compose f g =>
-    (* (TermDom g =? dom) &&& *)
-    (* (TermCod f =? cod) &&& *)
-    (TermCod g =? TermDom f) &&&
-    Term_well_typed_bool cat (TermCod g) cod f &&&
-    Term_well_typed_bool cat dom (TermCod g) g
+    (Fin.eqb (TermCod g) (TermDom f)) &&&
+    Term_well_typed_bool (TermCod g) cod f &&&
+    Term_well_typed_bool dom (TermCod g) g
   end.
 
-Lemma Term_well_typed_bool_sound cat dom cod e :
-  Term_well_typed_bool cat dom cod e = true <-> Term_well_typed cat dom cod e.
+Lemma Term_well_typed_bool_sound dom cod e :
+  Term_well_typed_bool dom cod e = true <-> Term_well_typed dom cod e.
 Proof.
   generalize dependent dom.
   generalize dependent cod.
-  induction e; simpl; intuition; equalities.
-  - apply Pos.eqb_refl.
+  induction e; simpl;
+  intuition; subst; equalities;
+  try rewrite !Fin_eqb_refl; auto.
   - apply IHe1; auto.
   - apply IHe2; auto.
   - apply IHe1 in H.
     apply IHe2 in H2.
-    rewrite H, H2; reflexivity.
+    rewrite !H0 in *.
+    rewrite Fin_eqb_refl, H, H2; reflexivity.
 Qed.
 
-Corollary Term_well_typed_cat {f cat dom cod } :
-  Term_well_typed cat dom cod f -> TermCat f = cat.
-Proof.
-  generalize dependent dom.
-  induction f; simpl; intros; intuition.
-  eapply IHf1; eauto.
-Qed.
-
-Corollary Term_well_typed_dom {f cat dom cod } :
-  Term_well_typed cat dom cod f -> TermDom f = dom.
+Corollary Term_well_typed_dom {f dom cod } :
+  Term_well_typed dom cod f -> TermDom f = dom.
 Proof.
   generalize dependent cod.
   induction f; simpl; intros; intuition.
   eapply IHf2; eauto.
 Qed.
 
-Corollary Term_well_typed_cod {f cat dom cod} :
-  Term_well_typed cat dom cod f -> TermCod f = cod.
+Corollary Term_well_typed_cod {f dom cod} :
+  Term_well_typed dom cod f -> TermCod f = cod.
 Proof.
   generalize dependent dom.
   induction f; simpl; intros; intuition.
@@ -648,8 +620,8 @@ Qed.
 
 Fixpoint normalize (p : Term) : ArrowList :=
   match p with
-  | Identity c x  => IdentityOnly c x
-  | Morph c x y f => ArrowChain (Arr c x y f) []
+  | Identity x  => IdentityOnly x
+  | Morph f     => ArrowChain f []
   | Compose f g => ArrowList_append (normalize f) (normalize g)
   end.
 
@@ -658,9 +630,6 @@ Lemma ArrowList_append_cat f g :
   ArrowList_cat (ArrowList_append f g) = ArrowList_cat g.
 Proof.
   destruct g, f; simpl; intros; auto.
-  - destruct a; subst; reflexivity.
-  - destruct a; simpl.
-    assumption.
 Qed.
 
 Lemma ArrowList_append_dom f g :
@@ -668,11 +637,7 @@ Lemma ArrowList_append_dom f g :
   ArrowList_dom (ArrowList_append f g) = ArrowList_dom g.
 Proof.
   destruct g, f; simpl; intros; auto.
-  - destruct a; subst; reflexivity.
-  - destruct a; simpl.
-    rewrite last_app_cons.
-    rewrite last_cons.
-    reflexivity.
+  now rewrite last_app_cons, last_cons.
 Qed.
 
 Lemma ArrowList_append_cod f g :
@@ -680,49 +645,40 @@ Lemma ArrowList_append_cod f g :
   ArrowList_cod (ArrowList_append f g) = ArrowList_cod f.
 Proof.
   destruct f, g; simpl; intros; auto.
-  - destruct a; subst; reflexivity.
-  - destruct a0; reflexivity.
 Qed.
 
-Lemma ArrowList_normalize_cat_dom_cod_sound {p cat dom cod} :
-  Term_well_typed cat dom cod p ->
-  ArrowList_cat (normalize p) = cat /\
+Lemma ArrowList_normalize_dom_cod_sound {p dom cod} :
+  Term_well_typed dom cod p ->
   ArrowList_dom (normalize p) = dom /\
   ArrowList_cod (normalize p) = cod.
 Proof.
-  generalize dependent cat.
   generalize dependent dom.
   generalize dependent cod.
   induction p; simpl; intros; intuition; subst;
   rewrite H0 in H;
-  rewrite ArrowList_append_cat ||
   rewrite ArrowList_append_dom ||
   rewrite ArrowList_append_cod; auto;
-  specialize (IHp1 _ _ _ H);
-  specialize (IHp2 _ _ _ H2);
+  specialize (IHp1 _ _ H);
+  specialize (IHp2 _ _ H2);
   intuition; congruence.
 Qed.
 
 Corollary ArrowList_specific_sound p :
-  Term_well_typed (TermCat p) (TermDom p) (TermCod p) p ->
-  ArrowList_cat (normalize p) = TermCat p /\
+  Term_well_typed (TermDom p) (TermCod p) p ->
   ArrowList_dom (normalize p) = TermDom p /\
   ArrowList_cod (normalize p) = TermCod p.
-Proof. apply ArrowList_normalize_cat_dom_cod_sound. Qed.
+Proof. apply ArrowList_normalize_dom_cod_sound. Qed.
 
-Lemma ArrowList_id_left c x y :
-  ArrowList_cat y = c ->
-  ArrowList_append (IdentityOnly c x) y = y.
+Lemma ArrowList_id_left x y :
+  ArrowList_append (IdentityOnly x) y = y.
 Proof.
   simpl.
   destruct y; simpl; intros; subst; auto.
-  destruct a; reflexivity.
 Qed.
 
-Lemma ArrowList_id_right f c y :
-  ArrowList_cat f = c ->
+Lemma ArrowList_id_right f y :
   ArrowList_dom f = y ->
-  ArrowList_append f (IdentityOnly c y) = f.
+  ArrowList_append f (IdentityOnly y) = f.
 Proof.
   destruct f; simpl; intros; subst; auto.
 Qed.
@@ -734,23 +690,21 @@ Proof.
   destruct x, y, z; simpl; auto; intros;
   try destruct a;
   try destruct a0; subst; auto.
-  destruct a1; simpl in *.
-  rewrite <- app_assoc.
-  reflexivity.
+  now rewrite <- app_assoc.
 Qed.
 
 (* We show here that ArrowList morphisms are just one way of representing a
    free category. However, we still forget identities and which way
    composition was associated, so really it's a normalized free category. *)
-Program Definition ArrowList_Category (cat : cat_idx) : Category := {|
+Program Definition ArrowList_Category : Category := {|
   obj := obj_idx;
   hom := fun x y =>
-    ∃ l : ArrowList, ArrowList_well_typed cat x y l;
+    ∃ l : ArrowList, ArrowList_well_typed x y l;
   homset := fun x y => {| equiv := fun f g => `1 f = `1 g |};
-  id := fun x => (IdentityOnly cat x; _);
+  id := fun x => (IdentityOnly x; _);
   compose := fun _ _ _ f g => (ArrowList_append (`1 f) (`1 g); _);
-  id_left := fun _ y f => ArrowList_id_left cat y (`1 f) _;
-  id_right := fun x _ f => ArrowList_id_right (`1 f) cat _ _ _;
+  id_left := fun _ y f => ArrowList_id_left y (`1 f);
+  id_right := fun x _ f => ArrowList_id_right (`1 f) _ _;
   comp_assoc := fun x y z w f g h =>
     ArrowList_append_assoc (`1 f) (`1 g) (`1 h)
 |}.
@@ -762,16 +716,6 @@ Next Obligation.
 Qed.
 Next Obligation. proper; simpl in *; subst; reflexivity. Qed.
 Next Obligation.
-  apply ArrowList_well_typed_cat in X.
-  destruct f; simpl; auto.
-  destruct a; intuition.
-Qed.
-Next Obligation.
-  apply ArrowList_well_typed_cat in X.
-  destruct f; simpl; auto.
-  destruct a; intuition.
-Qed.
-Next Obligation.
   now apply ArrowList_well_typed_dom in X.
 Qed.
 Next Obligation. apply ArrowList_append_assoc; congruence. Qed.
@@ -780,22 +724,20 @@ Next Obligation. rewrite ArrowList_append_assoc; auto; congruence. Qed.
 
 (* In the category whose morphisms are Terms, homset equivalence is up to
    normalized terms. *)
-Program Definition Term_Category (cat : cat_idx) : Category := {|
+Program Definition Term_Category : Category := {|
   obj := obj_idx;
-  hom := fun x y => ∃ l : Term, Term_well_typed cat x y l;
+  hom := fun x y => ∃ l : Term, Term_well_typed x y l;
   homset := fun x y => {| equiv := fun f g =>
     normalize (`1 f) = normalize (`1 g) |};
-  id := fun x => (Identity cat x; _);
+  id := fun x => (Identity x; _);
   compose := fun _ _ _ f g => (Compose (`1 f) (`1 g); _);
-  id_left := fun _ y f => ArrowList_id_left cat y (normalize (`1 f)) _;
-  id_right := fun x _ f => ArrowList_id_right (normalize (`1 f)) cat _ _ _;
+  id_left := fun _ y f => ArrowList_id_left y (normalize (`1 f));
+  id_right := fun x _ f => ArrowList_id_right (normalize (`1 f)) _ _;
   comp_assoc := fun x y z w f g h =>
     ArrowList_append_assoc
       (normalize (`1 f)) (normalize (`1 g)) (normalize (`1 h))
 |}.
 Next Obligation.
-  pose proof (Term_well_typed_cat X).
-  pose proof (Term_well_typed_cat X0).
   pose proof (Term_well_typed_dom X).
   pose proof (Term_well_typed_dom X0).
   pose proof (Term_well_typed_cod X).
@@ -803,13 +745,7 @@ Next Obligation.
   destruct f, g; simpl in *; intuition idtac; congruence.
 Qed.
 Next Obligation.
-  eapply ArrowList_normalize_cat_dom_cod_sound; eauto.
-Qed.
-Next Obligation.
-  eapply ArrowList_normalize_cat_dom_cod_sound; eauto.
-Qed.
-Next Obligation.
-  eapply ArrowList_normalize_cat_dom_cod_sound; eauto.
+  eapply ArrowList_normalize_dom_cod_sound; eauto.
 Qed.
 Next Obligation.
   rewrite ArrowList_append_assoc; auto;
@@ -827,9 +763,9 @@ Next Obligation.
   equalities; congruence.
 Qed.
 
-Lemma ArrowList_well_typed_sound {f cat dom cod} :
-  Term_well_typed cat dom cod f
-    -> ArrowList_well_typed cat dom cod (normalize f).
+Lemma ArrowList_well_typed_sound {f dom cod} :
+  Term_well_typed dom cod f
+    -> ArrowList_well_typed dom cod (normalize f).
 Proof.
   generalize dependent dom.
   generalize dependent cod.
@@ -844,123 +780,84 @@ Qed.
 
 Set Transparent Obligations.
 
-Program Instance Term_to_ArrowList (cat : cat_idx) :
-  Term_Category cat ⟶ ArrowList_Category cat := {
+Program Instance Term_to_ArrowList :
+  Term_Category ⟶ ArrowList_Category := {
   fobj := fun x => x;
   fmap := fun x y f => (normalize _; _)
 }.
-Next Obligation. apply ArrowList_well_typed_sound; auto. Qed.
+Next Obligation. now apply ArrowList_well_typed_sound. Qed.
 
 Fixpoint denormalize (f : ArrowList) : Term :=
   match f with
-  | IdentityOnly c x  => Identity c x
-  | ArrowChain (Arr c x y f) xs =>
-    (fold_left (fun acc x => (fun y => Compose y x) \o acc)
-               (map (fun x => match x with
-                                Arr c x y f => Morph c x y f
-                              end) xs)
-               Datatypes.id) (Morph c x y f)
+  | IdentityOnly x => Identity x
+  | ArrowChain f xs =>
+    fold_left (fun acc x => (fun y => Compose y x) \o acc)
+              (map Morph xs) Datatypes.id (Morph f)
   end.
 
-Lemma normalize_denormalize {cat dom cod f} :
-  ArrowList_well_typed cat dom cod f
+Lemma normalize_denormalize {dom cod f} :
+  ArrowList_well_typed dom cod f
     -> normalize (denormalize f) = f.
 Proof.
   destruct f; auto.
   generalize dependent a.
   generalize dependent dom.
-  induction l using rev_ind; intros.
-    destruct a; auto.
+  induction l using rev_ind; intros; auto.
   rewrite <- ArrowList_append_chains at 2.
-    rewrite <- (IHl (Arrow_cod x)); clear IHl.
-      destruct a; simpl.
-      rewrite map_app.
-      rewrite fold_left_app.
-      simpl.
-      f_equal.
-      destruct x; reflexivity.
-    destruct a; simpl in *.
-    destruct H, H0, H1.
-    apply ForallAligned_app in H2.
-    destruct H2, H3.
-    intuition.
-      destruct (last l (Arr c o o0 a)) eqn:?.
-      simpl in H4.
-      intuition.
-      inversion H1; subst.
-      apply Forall_app in H8.
-      destruct H8.
-      symmetry.
-      now sapply (last_Forall _ _ _ _ _ Heqa0 H).
-    constructor; inversion H1; subst; auto.
-    now apply Forall_app in H8.
-  destruct a; simpl in *.
-  destruct H, H0.
-  destruct H1.
-  apply ForallAligned_app in H2.
-  destruct H2, H3; intuition.
+  - rewrite <- (IHl (get_arr_cod x)); clear IHl.
+    + simpl.
+      now rewrite map_app, fold_left_app.
+    + simpl in H |- *;
+      equalities.
+      * rewrite app_comm_cons in H1.
+        now apply ForallAligned_app in H1.
+      * rewrite app_comm_cons in H1.
+        now apply ForallAligned_app in H1.
+  - simpl in *; equalities.
+    rewrite app_comm_cons in H1.
+    now apply ForallAligned_app in H1.
 Qed.
 
-Theorem denormalize_well_typed cat dom cod f :
-  ArrowList_well_typed cat dom cod f
-    -> Term_well_typed cat dom cod (denormalize f).
+Theorem denormalize_well_typed dom cod f :
+  ArrowList_well_typed dom cod f
+    -> Term_well_typed dom cod (denormalize f).
 Proof.
   destruct f; auto.
   generalize dependent a.
   generalize dependent dom.
   induction l using rev_ind; intros.
-    destruct a; simpl in *; intuition.
-    now inversion H.
-  assert (ArrowList_well_typed cat (Arrow_cod x) cod (ArrowChain a l)). {
+    simpl in *; intuition.
+  assert (ArrowList_well_typed (get_arr_cod x) cod (ArrowChain a l)). {
     clear IHl.
-    destruct a; simpl in *.
-    destruct H, H0.
-    destruct H1.
-    apply ForallAligned_app in H2.
-    destruct H2, H3; subst.
-    rewrite last_app_cons in H0; simpl in H0.
-    destruct x; intuition; subst.
-      simpl in *.
-      destruct (last l (Arr c0 o cod a)) eqn:?; auto.
-      simpl in H4.
-      inversion H1; subst; split; auto.
-      apply Forall_app in H6.
-      symmetry.
-      now sapply (last_Forall _ _ _ _ _ Heqa1 (proj1 H6)).
-    inversion H1; subst.
-    constructor; auto.
-    now apply Forall_app in H6.
+    simpl in *; equalities.
+    - rewrite app_comm_cons in H1.
+      now apply ForallAligned_app in H1.
+    - rewrite app_comm_cons in H1.
+      now apply ForallAligned_app in H1.
   }
   rewrite <- ArrowList_append_chains.
-  - specialize (IHl (Arrow_cod x) a H0).
-    simpl in H, H0.
-    destruct x, a; simpl.
-    rewrite last_app_cons in H; simpl in H.
-    equalities; subst.
-    apply ForallAligned_app in H7.
+  - specialize (IHl (get_arr_cod x) a H0).
+    simpl in *.
+    equalities.
+    rewrite last_app_cons in H1; simpl in H1.
+    rewrite app_comm_cons in H4.
+    apply ForallAligned_app in H4.
     equalities.
     clear H0.
-    rewrite map_app.
-    rewrite fold_left_app.
-    simpl in *.
-    rewrite H7.
+    rewrite map_app, fold_left_app.
+    simpl.
+    rewrite H5.
     intuition; subst.
     + clear -H.
       induction l using rev_ind; simpl; auto.
-      rewrite map_app.
-      rewrite fold_left_app; simpl in *.
-      rewrite last_rcons in *.
-      now destruct x.
-    + induction l using rev_ind; simpl; auto.
-    + now inversion H2.
-  - destruct a; simpl in *.
-    equalities; subst.
-    apply ForallAligned_app in H6.
-    equalities; intuition.
+      rewrite map_app, fold_left_app; simpl.
+      now rewrite last_rcons in *.
+    + now rewrite H5 in IHl.
+  - simpl in *; intuition.
 Qed.
 
-Program Instance ArrowList_to_Term (cat : cat_idx) :
-  ArrowList_Category cat ⟶ Term_Category cat := {
+Program Instance ArrowList_to_Term :
+  ArrowList_Category ⟶ Term_Category := {
   fobj := fun x => x;
   fmap := fun x y f => (denormalize (`1 f); _)
 }.
@@ -977,47 +874,24 @@ Next Obligation.
   eapply ArrowList_append_well_typed; eauto.
 Qed.
 
-Record Environment := {
-  cats : cat_idx -> Category;
-  objs : obj_idx -> ∀ c : cat_idx, cats c;
-  arrs : arr_idx -> ∀ (c : cat_idx) (a b : obj_idx),
-           option (objs a c ~{cats c}~> objs b c)
-}.
+Fixpoint denote dom cod (e : Term) :
+  option (get_obj dom ~{ vars_cat (get_cat c) }~> get_obj cod).
+Proof.
+  destruct e as [o|a|f g].
+  - destruct (Fin.eq_dec o dom); [|exact None].
+    destruct (Fin.eq_dec o cod); [|exact None].
+    subst; exact (Some id).
+  - destruct (Fin.eq_dec (get_arr_dom a) dom); [|exact None].
+    destruct (Fin.eq_dec (get_arr_cod a) cod); [|exact None].
+    subst; exact (Some (get_arr a)).
+  - destruct (denote (TermCod g) cod f); [|exact None].
+    destruct (denote dom (TermCod g) g); [|exact None].
+    exact (Some (h ∘ h0)).
+Defined.
 
-Variable env : Environment.
-
-Fixpoint denote cat dom cod (e : Term) :
-  option (objs env dom cat ~> objs env cod cat) :=
-  match e with
-  | Identity cat' t =>
-    match Pos.eq_dec cat cat',
-          Pos.eq_dec t dom, Pos.eq_dec t cod with
-    | left pf_cat, left pf_dom, left pf_cod =>
-      Some (match pf_cat, pf_dom, pf_cod with
-            | eq_refl, eq_refl, eq_refl =>
-              @id (cats env cat) (objs env t cat)
-            end)
-    | _, _ , _ => None
-    end
-  | Morph cat' dom' cod' n =>
-    match Pos.eq_dec cat cat',
-          Pos.eq_dec dom' dom, Pos.eq_dec cod' cod, arrs env n cat dom' cod' with
-    | left pf_cat, left pf_dom, left pf_cod, Some arr =>
-      Some (match pf_cat, pf_dom, pf_cod with
-            | eq_refl, eq_refl, eq_refl => arr
-            end)
-    | _, _, _, _ => None
-    end
-  | Compose g f =>
-    match denote cat dom (TermCod f) f, denote cat _ cod g with
-    | Some farr, Some garr => Some (garr ∘ farr)
-    | _ , _ => None
-    end
-  end.
-
-Lemma denote_cat_dom_cod {f cat dom cod f'} :
-  denote cat dom cod f = Some f' ->
-  TermCat f = cat /\ TermDom f = dom /\ TermCod f = cod.
+Lemma denote_dom_cod {f dom cod f'} :
+  denote dom cod f = Some f' ->
+  TermDom f = dom /\ TermCod f = cod.
 Proof.
   generalize dependent cod.
   generalize dependent dom.
@@ -1026,62 +900,58 @@ Proof.
   specialize (IHf1 (TermCod f2) cod).
   equalities.
   intros.
-  destruct (denote cat dom (TermCod f2) f2) eqn:?; try discriminate.
-  destruct (denote cat (TermCod f2) cod f1) eqn:?; try discriminate.
+  destruct (denote (TermCod f2) cod f1) eqn:?; try discriminate.
+  destruct (denote dom (TermCod f2) f2) eqn:?; try discriminate.
   destruct (IHf1 _ eq_refl).
   destruct (IHf2 _ eq_refl).
-  tauto.
+  intuition.
 Qed.
 
-Definition Term_well_defined cat dom cod (e : Term) : Type :=
-  ∃ f, denote cat dom cod e = Some f.
+Definition Term_well_defined dom cod (e : Term) : Type :=
+  ∃ f, denote dom cod e = Some f.
 
-Theorem Term_well_defined_is_well_typed {e cat dom cod} :
-  Term_well_defined cat dom cod e ->
-  Term_well_typed cat dom cod e.
+Theorem Term_well_defined_is_well_typed {e dom cod} :
+  Term_well_defined dom cod e ->
+  Term_well_typed dom cod e.
 Proof.
-  generalize dependent dom.
   generalize dependent cod.
-  generalize dependent cat.
+  generalize dependent dom.
   induction e; simpl in *;
-  intros cat dom cod [f H]; simpl in H.
-  - revert H; equalities.
-  - revert H; equalities.
-  - destruct (denote cat _ _ e2) eqn:?; try discriminate.
-    destruct (denote cat _ _ e1) eqn:?; try discriminate.
-    specialize (IHe1 cat dom (TermCod e2) (h0; Heqo0)).
-    specialize (IHe2 cat (TermCod e2) cod (h; Heqo)).
-    intuition.
-    symmetry.
-    eapply Term_well_typed_dom; eauto.
+  intros dom cod [f H]; simpl in H; equalities.
+  destruct (denote _ _ e1) eqn:?; try discriminate.
+  destruct (denote _ _ e2) eqn:?; try discriminate.
+  specialize (IHe1 (TermCod e2) cod (h; Heqo)).
+  specialize (IHe2 dom (TermCod e2) (h0; Heqo0)).
+  intuition.
+  symmetry.
+  eapply Term_well_typed_dom; eauto.
 Qed.
 
-Lemma denote_well_typed {p cat dom cod f} :
-  denote cat dom cod p = Some f -> Term_well_typed cat dom cod p.
+Lemma denote_well_typed {p dom cod f} :
+  denote dom cod p = Some f -> Term_well_typed dom cod p.
 Proof.
   generalize dependent f.
   generalize dependent dom.
   generalize dependent cod.
-  generalize dependent cat.
   induction p; simpl; intros ????; equalities.
-  destruct (denote cat _ _ p2) eqn:?.
-    destruct (denote cat _ _ p1) eqn:?.
-      pose proof (denote_cat_dom_cod Heqo).
-      pose proof (denote_cat_dom_cod Heqo0).
-      firstorder eauto.
-    intros; discriminate.
-  intros; discriminate.
+  destruct (denote _ _ p2) eqn:?;
+  destruct (denote _ _ p1) eqn:?; intros; try discriminate.
+  pose proof (denote_dom_cod Heqo).
+  pose proof (denote_dom_cod Heqo0).
+  intuition.
+    eapply IHp1; eauto.
+  eapply IHp2; eauto.
 Qed.
 
-Program Definition TermDef_Category (cat : cat_idx) : Category := {|
+Program Definition TermDef_Category : Category := {|
   obj := obj_idx;
-  hom := fun x y => ∃ l : Term, Term_well_defined cat x y l;
+  hom := fun x y => ∃ l : Term, Term_well_defined x y l;
   homset := fun x y => {| equiv := fun f g =>
     normalize (`1 f) = normalize (`1 g) |};
-  id := fun x => (Identity cat x; _);
+  id := fun x => (Identity x; _);
   compose := fun _ _ _ f g => (Compose (`1 f) (`1 g); _);
-  id_left := fun _ y f => ArrowList_id_left cat y (normalize (`1 f)) _;
-  id_right := fun x _ f => ArrowList_id_right (normalize (`1 f)) cat _ _ _;
+  id_left := fun _ y f => ArrowList_id_left y (normalize (`1 f));
+  id_right := fun x _ f => ArrowList_id_right (normalize (`1 f)) _ _;
   comp_assoc := fun x y z w f g h =>
     ArrowList_append_assoc
       (normalize (`1 f)) (normalize (`1 g)) (normalize (`1 h))
@@ -1094,23 +964,13 @@ Next Obligation.
   unshelve eexists; eauto.
     exact (x0 ∘ x).
   simpl.
-  destruct (denote_cat_dom_cod e).
-  destruct (denote_cat_dom_cod e0).
+  destruct (denote_dom_cod e).
+  destruct (denote_dom_cod e0).
   equalities; subst.
-  rewrite H1.
-  rewrite e, e0.
-  reflexivity.
+  now rewrite e, e0.
 Defined.
 Next Obligation.
-  eapply ArrowList_normalize_cat_dom_cod_sound; eauto.
-  eapply Term_well_defined_is_well_typed; eauto.
-Qed.
-Next Obligation.
-  eapply ArrowList_normalize_cat_dom_cod_sound; eauto.
-  eapply Term_well_defined_is_well_typed; eauto.
-Qed.
-Next Obligation.
-  eapply ArrowList_normalize_cat_dom_cod_sound; eauto.
+  eapply ArrowList_normalize_dom_cod_sound; eauto.
   eapply Term_well_defined_is_well_typed; eauto.
 Qed.
 Next Obligation.
@@ -1129,20 +989,20 @@ Next Obligation.
   equalities; congruence.
 Qed.
 
-Fixpoint normalize_denote_chain cat dom cod
+Fixpoint normalize_denote_chain dom cod
          (g : Arrow) (gs : list Arrow) {struct gs} :
-  option (objs env dom cat ~{ cats env cat }~> objs env cod cat) :=
+  option (get_obj dom ~{ vars_cat (get_cat c) }~> get_obj cod) :=
   match g, gs with
-  | Arr c x y h, nil =>
-    match arrs env h c x y with
+  | h, nil =>
+    match get_arr h with
     | Some p =>
       match Pos.eq_dec c cat,
             Pos.eq_dec x dom, Pos.eq_dec y cod with
       | left Hcat, left Hdom, left Hcod =>
-        Some (eq_rect y (fun z => objs env dom cat ~> objs env z cat)
-                      (eq_rect x (fun z => objs env z cat ~> objs env y cat)
+        Some (eq_rect y (fun z => objs env dom ~> objs env z cat)
+                      (eq_rect x (fun z => objs env z ~> objs env y cat)
                                (eq_rect c (fun c => objs env x c ~> objs env y c)
-                                        p cat Hcat) dom Hdom) cod Hcod)
+                                        p Hcat) dom Hdom) cod Hcod)
       | _, _, _ => None
       end
     | _ => None
@@ -1152,11 +1012,11 @@ Fixpoint normalize_denote_chain cat dom cod
     | Some p =>
       match Pos.eq_dec c1 cat, Pos.eq_dec y cod with
       | left Hcat, left Hcod =>
-        match normalize_denote_chain cat dom x (Arr c2 z w j) js with
+        match normalize_denote_chain dom x (Arr c2 z w j) js with
         | Some q =>
-          Some (eq_rect y (fun y => objs env dom cat ~> objs env y cat)
+          Some (eq_rect y (fun y => objs env dom ~> objs env y cat)
                         (eq_rect c1 (fun c => objs env x c ~> objs env y c)
-                                 p cat Hcat ∘ q) cod Hcod)
+                                 p Hcat ∘ q) cod Hcod)
         | _ => None
         end
       | _, _ => None
@@ -1166,9 +1026,9 @@ Fixpoint normalize_denote_chain cat dom cod
   end.
 
 Lemma normalize_denote_chain_cat :
-  ∀ (gs : list Arrow) c x y f cat dom cod f',
-    normalize_denote_chain cat dom cod (Arr c x y f) gs = Some f' ->
-    cat = c.
+  ∀ (gs : list Arrow) c x y f dom cod f',
+    normalize_denote_chain dom cod (Arr c x y f) gs = Some f' ->
+    = c.
 Proof.
   destruct gs; simpl; intros.
     destruct (arrs _ _ _).
@@ -1180,8 +1040,8 @@ Proof.
 Qed.
 
 Lemma normalize_denote_chain_cod :
-  ∀ (gs : list Arrow) c x y f cat dom cod f',
-    normalize_denote_chain cat dom cod (Arr c x y f) gs = Some f' ->
+  ∀ (gs : list Arrow) c x y f dom cod f',
+    normalize_denote_chain dom cod (Arr c x y f) gs = Some f' ->
     cod = y.
 Proof.
   destruct gs; simpl; intros.
@@ -1193,13 +1053,13 @@ Proof.
   revert H; equalities.
 Qed.
 
-Theorem normalize_denote_chain_compose {x xs y ys cat dom cod f} :
-  normalize_denote_chain cat dom cod x (xs ++ y :: ys) = Some f ->
+Theorem normalize_denote_chain_compose {x xs y ys dom cod f} :
+  normalize_denote_chain dom cod x (xs ++ y :: ys) = Some f ->
   ∃ mid g h, f ≈ g ∘ h ∧
-    Arrow_dom (last xs x) = mid ∧
-    Arrow_cod y = mid ∧
-    normalize_denote_chain cat mid cod x xs = Some g ∧
-    normalize_denote_chain cat dom mid y ys = Some h.
+    get_arr_dom (last xs x) = mid ∧
+    get_arr_cod y = mid ∧
+    normalize_denote_chain mid cod x xs = Some g ∧
+    normalize_denote_chain dom mid y ys = Some h.
 Proof.
   generalize dependent f.
   generalize dependent cod.
@@ -1208,7 +1068,7 @@ Proof.
   destruct x, x0, y; simpl.
   - destruct (arrs _ _ _); try discriminate.
     revert H; equalities.
-    destruct (normalize_denote_chain cat dom o1 (Arr c1 o3 o4 a1) ys) eqn:?;
+    destruct (normalize_denote_chain dom o1 (Arr c1 o3 o4 a1) ys) eqn:?;
     try discriminate.
     exists _, h, h0.
     inversion_clear H.
@@ -1217,7 +1077,7 @@ Proof.
     pose proof (normalize_denote_chain_cod _ _ _ _ _ _ _ _ _ Heqo2); auto.
   - destruct (arrs _ _ _) eqn:?; try discriminate.
     revert H; equalities.
-    destruct (normalize_denote_chain cat dom o1 (Arr c1 o3 o4 a1)
+    destruct (normalize_denote_chain dom o1 (Arr c1 o3 o4 a1)
                                      (l ++ y0 :: ys)) eqn:?;
     try discriminate.
     destruct (X _ _ _ Heqo2), s, s.
@@ -1245,10 +1105,10 @@ Proof.
     + now rewrite a4.
 Admitted.
 
-Lemma normalize_denote_chain_cat_dom_cod :
-  ∀ (gs : list Arrow) c x y f cat dom cod f',
-    normalize_denote_chain cat dom cod (Arr c x y f) gs = Some f' ->
-    cat = c /\
+Lemma normalize_denote_chain_dom_cod :
+  ∀ (gs : list Arrow) c x y f dom cod f',
+    normalize_denote_chain dom cod (Arr c x y f) gs = Some f' ->
+    = c /\
     cod = y /\
     dom = match last gs (Arr c x y f) with Arr _ z _ _ => z end.
 Proof.
@@ -1268,9 +1128,9 @@ Proof.
   intuition.
 Qed.
 
-Theorem normalize_denote_chain_append_dom_cod : ∀ x xs y ys cat dom cod f,
-  normalize_denote_chain cat dom cod x (xs ++ y :: ys) = Some f ->
-  Arrow_dom (last xs x) = Arrow_cod y.
+Theorem normalize_denote_chain_append_dom_cod : ∀ x xs y ys dom cod f,
+  normalize_denote_chain dom cod x (xs ++ y :: ys) = Some f ->
+  get_arr_dom (last xs x) = get_arr_cod y.
 Proof.
   intros.
   destruct (normalize_denote_chain_compose H).
@@ -1280,26 +1140,26 @@ Proof.
 Qed.
 
 (* The list [f; g; h] maps to [f ∘ g ∘ h]. *)
-Definition normalize_denote cat dom cod (xs : ArrowList) :
-  option (objs env dom cat ~> objs env cod cat) :=
+Definition normalize_denote dom cod (xs : ArrowList) :
+  option (objs env dom ~> objs env cod cat) :=
   match xs with
   | IdentityOnly c x =>
     match Pos.eq_dec c cat,
           Pos.eq_dec x dom, Pos.eq_dec x cod with
     | left Hcat, left Hdom, left Hcod =>
-      Some (eq_rect x (fun z => objs env dom cat ~> objs env z cat)
-              (eq_rect x (fun z => objs env z cat ~> objs env x cat)
+      Some (eq_rect x (fun z => objs env dom ~> objs env z cat)
+              (eq_rect x (fun z => objs env z ~> objs env x cat)
                  (eq_rect c (fun z => objs env x z ~> objs env x z)
-                          (@id (cats env c) (objs env x c)) cat Hcat)
+                          (@id (cats env c) (objs env x c)) Hcat)
                  dom Hdom)
               cod Hcod)
     | _, _, _ => None
     end
-  | ArrowChain f fs => normalize_denote_chain cat dom cod f fs
+  | ArrowChain f fs => normalize_denote_chain dom cod f fs
   end.
 
-Theorem normalize_list_cat {p cat dom cod f} :
-  normalize_denote cat dom cod p = Some f -> ArrowList_cat p = cat.
+Theorem normalize_list_cat {p dom cod f} :
+  normalize_denote dom cod p = Some f -> ArrowList_cat p = cat.
 Proof.
   intros.
   destruct p.
@@ -1316,8 +1176,8 @@ Proof.
     destruct (arrs _ _ _ _); discriminate.
 Qed.
 
-Theorem normalize_list_cod {p cat dom cod f} :
-  normalize_denote cat dom cod p = Some f -> ArrowList_cod p = cod.
+Theorem normalize_list_cod {p dom cod f} :
+  normalize_denote dom cod p = Some f -> ArrowList_cod p = cod.
 Proof.
   intros.
   destruct p.
@@ -1334,8 +1194,8 @@ Proof.
     destruct (arrs _ _ _ _); discriminate.
 Qed.
 
-Theorem normalize_list_dom {p cat dom cod f} :
-  normalize_denote cat dom cod p = Some f -> ArrowList_dom p = dom.
+Theorem normalize_list_dom {p dom cod f} :
+  normalize_denote dom cod p = Some f -> ArrowList_dom p = dom.
 Proof.
   generalize dependent f.
   generalize dependent cod.
@@ -1349,7 +1209,7 @@ Proof.
     destruct a1, a2.
     destruct (arrs _ _ _); try discriminate.
     revert H; equalities.
-    destruct (normalize_denote_chain cat dom o (Arr c0 o1 o2 a0) l) eqn:Heqe;
+    destruct (normalize_denote_chain dom o (Arr c0 o1 o2 a0) l) eqn:Heqe;
     try discriminate.
     rewrite <- (IHp _ _ Heqe); clear IHp.
     induction l using rev_ind.
@@ -1360,28 +1220,28 @@ Proof.
     destruct l; auto.
 Qed.
 
-Theorem normalize_denote_well_typed {p cat dom cod f} :
-  normalize_denote cat dom cod p = Some f
-    -> ∃ p', p = normalize p' ∧ Term_well_typed cat dom cod p'.
+Theorem normalize_denote_well_typed {p dom cod f} :
+  normalize_denote dom cod p = Some f
+    -> ∃ p', p = normalize p' ∧ Term_well_typed dom cod p'.
 Proof.
   generalize dependent f.
   generalize dependent cod.
   induction p using ArrowList_list_rect; simpl; intros.
   - revert H; equalities.
-    exists (Identity cat cod).
+    exists (Identity cod).
     simpl; intuition.
   - destruct a.
     destruct (arrs _ _ _); try discriminate.
     revert H; equalities.
-    exists (Morph cat dom cod a).
+    exists (Morph dom cod a).
     simpl; intuition.
   - destruct a1, a2.
     destruct (arrs _ _ _); try discriminate.
     revert H; equalities.
-    destruct (normalize_denote_chain cat dom o (Arr c0 o1 o2 a0) l) eqn:?;
+    destruct (normalize_denote_chain dom o (Arr c0 o1 o2 a0) l) eqn:?;
     try discriminate.
     destruct (IHp _ _ Heqo0), p.
-    exists (Compose (Morph cat o cod a) x).
+    exists (Compose (Morph o cod a) x).
     simpl.
     inversion_clear H.
     intuition.
@@ -1393,15 +1253,15 @@ Proof.
     + erewrite Term_well_typed_cod; eauto.
 Qed.
 
-Theorem normalize_compose {x y cat dom cod f} :
+Theorem normalize_compose {x y dom cod f} :
   ArrowList_cat y = ArrowList_cat x ->
   ArrowList_cod y = ArrowList_dom x ->
-  normalize_denote cat dom cod (ArrowList_append x y) = Some f ->
+  normalize_denote dom cod (ArrowList_append x y) = Some f ->
   ∃ mid g h, f ≈ g ∘ h ∧
     ArrowList_dom x = mid ∧
     ArrowList_cod y = mid ∧
-    normalize_denote cat mid cod x = Some g ∧
-    normalize_denote cat dom mid y = Some h.
+    normalize_denote mid cod x = Some g ∧
+    normalize_denote dom mid y = Some h.
 Proof.
   generalize dependent f.
   generalize dependent cod.
@@ -1446,10 +1306,10 @@ Proof.
       apply (normalize_denote_chain_compose H1).
 Qed.
 
-Theorem normalize_sound {p cat dom cod f} :
-  Term_well_typed cat dom cod p ->
-  normalize_denote cat dom cod (normalize p) = Some f ->
-  ∃ f', f ≈ f' ∧ denote cat dom cod p = Some f'.
+Theorem normalize_sound {p dom cod f} :
+  Term_well_typed dom cod p ->
+  normalize_denote dom cod (normalize p) = Some f ->
+  ∃ f', f ≈ f' ∧ denote dom cod p = Some f'.
 Proof.
   generalize dependent dom.
   generalize dependent cod.
@@ -1473,36 +1333,36 @@ Proof.
         exists (x2 ∘ x3).
         split; auto.
         now rewrite <- e0, <- e2.
-      * pose proof (ArrowList_normalize_cat_dom_cod_sound H2);
+      * pose proof (ArrowList_normalize_dom_cod_sound H2);
         equalities;
         now rewrite a1 in H4.
     + clear IHp1 IHp2.
       equalities.
-      pose proof (ArrowList_normalize_cat_dom_cod_sound H2).
-      pose proof (ArrowList_normalize_cat_dom_cod_sound H3).
+      pose proof (ArrowList_normalize_dom_cod_sound H2).
+      pose proof (ArrowList_normalize_dom_cod_sound H3).
       equalities.
       now rewrite H4.
     + clear IHp1 IHp2.
       equalities.
-      pose proof (ArrowList_normalize_cat_dom_cod_sound H2).
-      pose proof (ArrowList_normalize_cat_dom_cod_sound H3).
+      pose proof (ArrowList_normalize_dom_cod_sound H2).
+      pose proof (ArrowList_normalize_dom_cod_sound H3).
       equalities.
       now rewrite H5, H7.
 Qed.
 
-Theorem normalize_apply cat dom cod : ∀ f g,
-  Term_well_typed_bool cat dom cod f = true ->
-  Term_well_typed_bool cat dom cod g = true ->
+Theorem normalize_apply dom cod : ∀ f g,
+  Term_well_typed_bool dom cod f = true ->
+  Term_well_typed_bool dom cod g = true ->
   ArrowList_beq (normalize f) (normalize g) = true ->
-  normalize_denote cat dom cod (normalize f) ||| false = true ->
-  denote cat dom cod f ≈ denote cat dom cod g.
+  normalize_denote dom cod (normalize f) ||| false = true ->
+  denote dom cod f ≈ denote dom cod g.
 Proof.
   intros.
   apply Term_well_typed_bool_sound in H.
   apply Term_well_typed_bool_sound in H0.
   pose proof (ArrowList_well_typed_sound H).
   apply ArrowList_beq_eq in H1.
-  destruct (normalize_denote cat dom cod (normalize f)) eqn:?;
+  destruct (normalize_denote dom cod (normalize f)) eqn:?;
   try discriminate.
   destruct (normalize_sound H Heqo), p.
   rewrite e0; clear e0.
@@ -1514,20 +1374,20 @@ Proof.
   reflexivity.
 Qed.
 
-Corollary normalize_denote_terms cat dom cod : ∀ f g,
-  Term_well_typed_bool cat dom cod f = true ->
-  Term_well_typed_bool cat dom cod g = true ->
+Corollary normalize_denote_terms dom cod : ∀ f g,
+  Term_well_typed_bool dom cod f = true ->
+  Term_well_typed_bool dom cod g = true ->
   ArrowList_beq (normalize f) (normalize g) = true ->
-  normalize_denote cat dom cod (normalize f) ||| false = true ->
-  normalize_denote cat dom cod (normalize f)
-    ≈ normalize_denote cat dom cod (normalize g) ->
-  denote cat dom cod f ≈ denote cat dom cod g.
+  normalize_denote dom cod (normalize f) ||| false = true ->
+  normalize_denote dom cod (normalize f)
+    ≈ normalize_denote dom cod (normalize g) ->
+  denote dom cod f ≈ denote dom cod g.
 Proof. intros; apply normalize_apply; auto. Qed.
 
-Corollary normalize_denote_terms_impl cat dom cod : ∀ f g,
+Corollary normalize_denote_terms_impl dom cod : ∀ f g,
   ArrowList_beq (normalize f) (normalize g) = true ->
-  normalize_denote cat dom cod (normalize f)
-    ≈ normalize_denote cat dom cod (normalize g).
+  normalize_denote dom cod (normalize f)
+    ≈ normalize_denote dom cod (normalize g).
 Proof.
   intros.
   apply ArrowList_beq_eq in H.
@@ -1809,8 +1669,8 @@ Hint Resolve denormalize_well_typed.
 
    Since the objects of both categories are the same, the monad this gives
    rise to is uninteresting. *)
-Program Instance Term_ArrowList_Adjunction (cat : cat_idx) :
-  ArrowList_to_Term cat ⊣ Term_to_ArrowList cat := {
+Program Instance Term_ArrowList_Adjunction :
+  ArrowList_to_Term ⊣ Term_to_ArrowList := {
   adj := fun x y =>
     {| to   := {| morphism := fun f => (normalize (_ f); _) |}
      ; from := {| morphism := _ |} |}
